Untyped view of references

ulib/FStar.Monotonic.Heap.fst
@@ -22,17 +22,17 @@ let emp = {
   memory    = (fun (r:nat) -> None)
 }
 
-private type mref' (a:Type0) (rel:preorder a) :Type0 = {
+private noeq type mref' (a:Type0) (rel:preorder a) :Type0 = {
   addr: nat;
-  init: a;
-  mm:   bool;  //manually managed flag
+  init: FStar.Ghost.erased a;
+  mm:   FStar.Ghost.erased bool;  //manually managed flag
 }
 
 let mref a rel = mref' a rel
 
 let addr_of #a #rel r = r.addr
 
-let is_mm #a #rel r = r.mm
+let is_mm #a #rel r = FStar.Ghost.reveal r.mm
 
 let compare_addrs #a #b #rel1 #rel2 r1 r2 = r1.addr = r2.addr
 
@@ -53,16 +53,18 @@ let sel_tot #a #rel h r =
 let sel #a #rel h r =
   if FStar.StrongExcludedMiddle.strong_excluded_middle (h `contains` r) then
     sel_tot #a h r
-  else r.init
+  else FStar.Ghost.reveal r.init
 
-let upd_tot #a #rel h r x =
+let upd_tot' (#a: Type0) (#rel: preorder a) (h: heap) (r: mref a rel) (x: a) =
   { h with memory = (fun r' -> if r.addr = r'
 			    then Some (| a, Some rel, x |)
                             else h.memory r') }
 
+let upd_tot #a #rel h r x = upd_tot' h r x
+
 let upd #a #rel h r x =
   if FStar.StrongExcludedMiddle.strong_excluded_middle (h `contains` r)
-  then upd_tot h r x
+  then upd_tot' h r x
   else
     if r.addr >= h.next_addr
     then
@@ -76,7 +78,7 @@ let upd #a #rel h r x =
                                 else h.memory r') }
 
 let alloc #a rel h x mm =
-  let r = { addr = h.next_addr; init = x; mm = mm } in
+  let r = { addr = h.next_addr; init = FStar.Ghost.hide x; mm = FStar.Ghost.hide mm } in
   r, { next_addr = r.addr + 1;
        memory    = (fun (r':nat) -> if r' = r.addr
 	   		        then Some (| a, Some rel, x |)
@@ -168,6 +170,8 @@ let lemma_free_mm_sel #a #b #rel1 #rel2 h0 r1 r2 = ()
 let lemma_free_mm_contains #a #b #rel1 #rel2 h0 r1 r2 = ()
 let lemma_free_mm_unused #a #b #rel1 #rel2 h0 r1 r2 = ()
 let lemma_sel_same_addr #a #rel h r1 r2 = ()
+let lemma_upd_same_addr #a #rel h r1 r2 x =
+  assert (equal (upd h r1 x) (upd h r2 x))
 let lemma_sel_upd1 #a #rel h r1 x r2 = ()
 let lemma_sel_upd2 #a #b #rel1 #rel2 h r1 r2 x = ()
 let lemma_mref_injectivity = ()
@@ -183,3 +187,78 @@ let lemma_unused_upd_modifies #a #rel h r x = ()
 let upd_upd_same_mref #a #rel h r x y = assert (equal (upd (upd h r x) r y) (upd h r y))
 let lemma_sel_equals_sel_tot_for_contained_refs #a #rel h r = ()
 let lemma_upd_equals_upd_tot_for_contained_refs #a #rel h r x = ()
+
+
+(*** Untyped views of references *)
+
+(* Definition and ghost decidable equality *)
+noeq type aref' :Type0 = {
+  a_addr: nat;
+  a_mm:   FStar.Ghost.erased bool;  //manually managed flag
+}
+let aref = aref'
+let dummy_aref = {
+  a_addr = 0;
+  a_mm   = FStar.Ghost.hide false;
+}
+let aref_equal a1 a2 = a1.a_addr = a2.a_addr && FStar.Ghost.reveal a1.a_mm = FStar.Ghost.reveal a2.a_mm
+
+(* Introduction rule *)
+let aref_of #t #rel r = {
+  a_addr = r.addr;
+  a_mm   = r.mm;
+}
+
+(* Operators lifted from ref *)
+let addr_of_aref a = a.a_addr
+let addr_of_aref_of #t #rel r = ()
+let aref_is_mm a = FStar.Ghost.reveal a.a_mm
+let is_mm_aref_of #t #rel r = ()
+let aref_unused_in a h = None? (h.memory a.a_addr)
+let unused_in_aref_of #t #rel r h = ()
+let contains_aref_unused_in #a #rel h x y = ()
+
+(* Elimination rule *)
+let aref_live_at (h: heap) (a: aref) (t: Type0) (rel: preorder t) =
+  let _ = () in
+  Some? (h.memory a.a_addr) /\
+  (let Some (| a1, pre_opt, _ |) = h.memory a.a_addr in
+   t == a1 /\ Some? pre_opt /\ Some?.v pre_opt === rel)  //using `===` here, since otherwise typechecker fails with a and a1 being different types, why?
+
+let ref_of'
+  (h: heap)
+  (a: aref)
+  (t: Type0)
+  (rel: preorder t)
+: Pure (mref t rel)
+  (requires (aref_live_at h a t rel))
+  (ensures (fun _ -> True))
+= let Some (| _, pre_opt, x |) = h.memory a.a_addr in
+  {
+    addr = a.a_addr;
+    init = FStar.Ghost.hide x;
+    mm = a.a_mm
+  }
+
+let gref_of a t rel =
+  let m : squash (exists (h: heap) . aref_live_at h a t rel) = () in
+  let l : (exists (h: heap) . aref_live_at h a t rel) =
+    Squash.join_squash #(h: heap & aref_live_at h a t rel) m
+  in
+  let k : (exists (h: heap { aref_live_at h a t rel} ) . squash True ) =
+    FStar.Squash.bind_squash
+      #(h: heap & aref_live_at h a t rel)
+      #(h: (h: heap { aref_live_at h a t rel} ) & squash True)
+      l
+      (fun h -> let (| h', _ |) = h in Squash.return_squash (| h', () |) )
+  in
+  let h = FStar.ErasedLogic.exists_proj1 #(h: heap {aref_live_at h a t rel}) #(fun _ -> squash True) k in
+  ref_of' h a t rel
+
+let ref_of h a t rel = ref_of' h a t rel
+
+let aref_live_at_aref_of h #t #rel r = ()
+let contains_gref_of h a t rel = ()
+let aref_of_gref_of a t rel = ()
+
+let _eof = ()
